src/MicroSail/Symbolic/Sound.v
@@ -66,215 +66,221 @@ Module Soundness
   Program Instance proper_sub_comp {Σ1 Σ2 Σ3} : Proper (eq ==> eq ==> eq) (@sub_comp Σ1 Σ2 Σ3).
   Admit Obligations.
 
-  Section Soundness.
+  Module DynMutV1Soundness.
 
-    Context `{HL: IHeaplet L} {SLL: ISepLogicLaws L}.
+    Import DynMutV1.
 
-    Definition inst_heap {Σ} (ι : SymInstance Σ) (h : SymbolicHeap Σ) : L :=
-      List.fold_right (fun c h => inst_chunk ι c ∧ h) ltrue h.
+    Section WithSemantics.
 
-    Axiom sub_comp_id_left : forall {Σ0 Σ1} (ζ : Sub Σ0 Σ1), sub_comp (sub_id Σ0) ζ = ζ.
-    Axiom sub_comp_id_right : forall {Σ0 Σ1} (ζ : Sub Σ0 Σ1), sub_comp ζ (sub_id Σ1) = ζ.
-    Axiom subst_sub_id : forall `{Subst T} Σ (t : T Σ), subst (sub_id _) t = t.
-    Axiom subst_sub_comp : forall `{Subst T} Σ0 Σ1 Σ2 (ζ1 : Sub Σ0 Σ1) (ζ2 : Sub Σ1 Σ2) t, subst (sub_comp ζ1 ζ2) t = subst ζ2 (subst ζ1 t).
-    Axiom sub_comp_comm : forall {Σ0 Σ1 Σ2 Σ3} (ζ1 : Sub Σ0 Σ1) (ζ2 : Sub Σ1 Σ2) (ζ3 : Sub Σ2 Σ3), sub_comp (sub_comp ζ1 ζ2) ζ3 = sub_comp ζ1 (sub_comp ζ2 ζ3).
+      Context `{HL: IHeaplet L} {SLL: ISepLogicLaws L}.
 
-    (* Lemma  *)
-    (* subst ζ'' (symbolic_eval_exp δ0 e) *)
-    (* = symbolic_eval_exp (inst_localstore ζ'' δ0) *)
+      Definition inst_heap {Σ} (ι : SymInstance Σ) (h : SymbolicHeap Σ) : L :=
+        List.fold_right (fun c h => inst_chunk ι c ∧ h) ltrue h.
 
-    Ltac sauto :=
-      repeat
+      Axiom sub_comp_id_left : forall {Σ0 Σ1} (ζ : Sub Σ0 Σ1), sub_comp (sub_id Σ0) ζ = ζ.
+      Axiom sub_comp_id_right : forall {Σ0 Σ1} (ζ : Sub Σ0 Σ1), sub_comp ζ (sub_id Σ1) = ζ.
+      Axiom subst_sub_id : forall `{Subst T} Σ (t : T Σ), subst (sub_id _) t = t.
+      Axiom subst_sub_comp : forall `{Subst T} Σ0 Σ1 Σ2 (ζ1 : Sub Σ0 Σ1) (ζ2 : Sub Σ1 Σ2) t, subst (sub_comp ζ1 ζ2) t = subst ζ2 (subst ζ1 t).
+      Axiom sub_comp_comm : forall {Σ0 Σ1 Σ2 Σ3} (ζ1 : Sub Σ0 Σ1) (ζ2 : Sub Σ1 Σ2) (ζ3 : Sub Σ2 Σ3), sub_comp (sub_comp ζ1 ζ2) ζ3 = sub_comp ζ1 (sub_comp ζ2 ζ3).
+
+      (* Lemma  *)
+      (* subst ζ'' (symbolic_eval_exp δ0 e) *)
+      (* = symbolic_eval_exp (inst_localstore ζ'' δ0) *)
+
+      Ltac sauto :=
+        repeat
+          match goal with
+          | [ |- ?P ⊢ ?P ] =>
+            apply entails_refl
+          | [ |- ?P ∧ _ ⊢ ?P ∧ _ ] =>
+            apply land_right; [ apply land_left1, entails_refl | idtac ]
+          | [ |- _ ⊢ _ ∧ !!(?x = ?x) ] =>
+            apply land_right; [ idtac | apply lprop_right; reflexivity ]
+          | [ |- !! _ ⊢ _ ] =>
+            apply lprop_right; intro
+          | [ H: ?P |- _ ⊢ !!?P ] =>
+            apply lprop_right; exact H
+          end.
+
+      Local Ltac sound_inster :=
         match goal with
-        | [ |- ?P ⊢ ?P ] =>
-          apply entails_refl
-        | [ |- ?P ∧ _ ⊢ ?P ∧ _ ] =>
-          apply land_right; [ apply land_left1, entails_refl | idtac ]
-        | [ |- _ ⊢ _ ∧ !!(?x = ?x) ] =>
-          apply land_right; [ idtac | apply lprop_right; reflexivity ]
-        | [ |- !! _ ⊢ _ ] =>
-          apply lprop_right; intro
-        | [ H: ?P |- _ ⊢ !!?P ] =>
-          apply lprop_right; exact H
+        | [ IH: outcome_satisfy (dmut_exec ?s _ _) |-
+            outcome_satisfy (dmut_exec ?s _ _) _ ] =>
+          refine (outcome_satisfy_monotonic _ _ IH); clear IH
+        | [ IH: context[_ -> outcome_satisfy (dmut_exec ?s _ _) _] |-
+            outcome_satisfy (dmut_exec ?s _ _) _ ] =>
+          microsail_insterU (fail) IH; refine (outcome_satisfy_monotonic _ _ IH); clear IH
         end.
 
-    Local Ltac sound_inster :=
-      match goal with
-      | [ IH: outcome_satisfy (dmut_exec ?s _ _) |-
-          outcome_satisfy (dmut_exec ?s _ _) _ ] =>
-        refine (outcome_satisfy_monotonic _ _ IH); clear IH
-      | [ IH: context[_ -> outcome_satisfy (dmut_exec ?s _ _) _] |-
-          outcome_satisfy (dmut_exec ?s _ _) _ ] =>
-        microsail_insterU (fail) IH; refine (outcome_satisfy_monotonic _ _ IH); clear IH
-      end.
+      Lemma subst_lookup {Γ Σ Σ' x σ} (xInΓ : (x ∶ σ)%ctx ∈ Γ) (ζ : Sub Σ Σ') (δ : SymbolicLocalStore Γ Σ) :
+        (subst ζ (δ ‼ x) = (subst ζ δ ‼ x))%lit.
+      Proof.
+        unfold subst at 2, sub_localstore.
+        now rewrite env_lookup_map.
+      Qed.
 
-    Lemma subst_lookup {Γ Σ Σ' x σ} (xInΓ : (x ∶ σ)%ctx ∈ Γ) (ζ : Sub Σ Σ') (δ : SymbolicLocalStore Γ Σ) :
-      (subst ζ (δ ‼ x) = (subst ζ δ ‼ x))%lit.
-    Proof.
-      unfold subst at 2, sub_localstore.
-      now rewrite env_lookup_map.
-    Qed.
+      Lemma subst_symboliceval {Γ τ Σ Σ'} (e : Exp Γ τ) (ζ : Sub Σ Σ') (δ : SymbolicLocalStore Γ Σ) :
+        subst (T := fun Σ => Term Σ _) ζ (symbolic_eval_exp δ e) = symbolic_eval_exp (subst ζ δ) e.
+      Proof.
+        induction e; cbn; f_equal; auto.
+        { now rewrite (subst_lookup xInΓ). }
+        all: induction es; cbn in *; destruct_conjs; f_equal; auto.
+      Qed.
 
-    Lemma subst_symboliceval {Γ τ Σ Σ'} (e : Exp Γ τ) (ζ : Sub Σ Σ') (δ : SymbolicLocalStore Γ Σ) :
-      subst (T := fun Σ => Term Σ _) ζ (symbolic_eval_exp δ e) = symbolic_eval_exp (subst ζ δ) e.
-    Proof.
-      induction e; cbn; f_equal; auto.
-      { now rewrite (subst_lookup xInΓ). }
-      all: induction es; cbn in *; destruct_conjs; f_equal; auto.
-    Qed.
-
-    Lemma eval_exp_inst {Γ Σ τ} (ι : SymInstance Σ) (δΓΣ : SymbolicLocalStore Γ Σ) (e : Exp Γ τ) :
-      eval e (inst_localstore ι δΓΣ) = inst_term ι (symbolic_eval_exp δΓΣ e).
-    Proof.
-      induction e; cbn; repeat f_equal; auto.
-      { unfold inst_localstore; now rewrite env_lookup_map. }
-      2: {
-        induction es as [|eb n es IHes]; cbn in *.
-        { reflexivity. }
-        { destruct X as [-> Heqs].
-          destruct (inst_term ι (symbolic_eval_exp δΓΣ eb));
-            cbn; f_equal; auto.
+      Lemma eval_exp_inst {Γ Σ τ} (ι : SymInstance Σ) (δΓΣ : SymbolicLocalStore Γ Σ) (e : Exp Γ τ) :
+        eval e (inst_localstore ι δΓΣ) = inst_term ι (symbolic_eval_exp δΓΣ e).
+      Proof.
+        induction e; cbn; repeat f_equal; auto.
+        { unfold inst_localstore; now rewrite env_lookup_map. }
+        2: {
+          induction es as [|eb n es IHes]; cbn in *.
+          { reflexivity. }
+          { destruct X as [-> Heqs].
+            destruct (inst_term ι (symbolic_eval_exp δΓΣ eb));
+              cbn; f_equal; auto.
+          }
         }
-      }
-      all: induction es; cbn in *; destruct_conjs; f_equal; auto.
-    Qed.
+        all: induction es; cbn in *; destruct_conjs; f_equal; auto.
+      Qed.
 
-    Local Opaque inst_heap.
+      Local Opaque inst_heap.
 
-    Opaque env_tail.
+      Opaque env_tail.
 
-    Notation "'dmutres_pathcondition' res" := (symbolicstate_pathcondition (mutator_result_state (dmutres_result res))) (at level 10).
-    Notation "'dmutres_heap' res" := (symbolicstate_heap (mutator_result_state (dmutres_result res))) (at level 10).
-    Notation "'dmutres_localstore' res" := (symbolicstate_localstore (mutator_result_state (dmutres_result res))) (at level 10).
+      Notation "'dmutres_pathcondition' res" := (symbolicstate_pathcondition (mutator_result_state (dmutres_result res))) (at level 10).
+      Notation "'dmutres_heap' res" := (symbolicstate_heap (mutator_result_state (dmutres_result res))) (at level 10).
+      Notation "'dmutres_localstore' res" := (symbolicstate_localstore (mutator_result_state (dmutres_result res))) (at level 10).
 
-    Lemma dmut_exec_sound {Γ σ} (POST : Lit σ -> LocalStore Γ -> L) (s : Stm Γ σ) :
-      forall Σ0 Σ1  (ι : SymInstance Σ1) (ζ1 : Sub Σ0 Σ1) (pc1 : PathCondition Σ1) (δ1 : SymbolicLocalStore Γ Σ1) (h1 : SymbolicHeap Σ1),
-        let δ       := inst_localstore ι δ1 in
-        let pre__pc   := !! inst_pathcondition ι pc1 in
-        let pre__heap := inst_heap ι h1 in
-        outcome_satisfy
-          (dmut_exec s ζ1 (MkSymbolicState pc1 δ1 h1))
-          (fun '(@MkDynMutResult _ _ _ Σ2 ζ2 (MkMutResult t (MkSymbolicState pc2 δ2 h2) x)) =>
-             forall (ι' : SymInstance Σ2),
-               ι = env_map (fun _ => inst_term ι') ζ2 ->
-               let post__pc   := !! inst_pathcondition ι' pc2 in
-               let post__heap := inst_heap ι' h2 in
-               post__pc ∧ post__heap ⊢ POST (inst_term ι' t) (inst_localstore ι' δ2)) ->
-        δ ⊢ ⦃ pre__pc ∧ pre__heap ⦄ s ⦃ POST ⦄.
-    Proof.
-      intros ? ? ? ? ? ? ?; cbn.
-      revert pc1 h1.
-      induction s.
+      Lemma dmut_exec_sound {Γ σ} (POST : Lit σ -> LocalStore Γ -> L) (s : Stm Γ σ) :
+        forall Σ0 Σ1  (ι : SymInstance Σ1) (ζ1 : Sub Σ0 Σ1) (pc1 : PathCondition Σ1) (δ1 : SymbolicLocalStore Γ Σ1) (h1 : SymbolicHeap Σ1),
+          let δ       := inst_localstore ι δ1 in
+          let pre__pc   := !! inst_pathcondition ι pc1 in
+          let pre__heap := inst_heap ι h1 in
+          outcome_satisfy
+            (dmut_exec s ζ1 (MkSymbolicState pc1 δ1 h1))
+            (fun '(@MkDynMutResult _ _ _ Σ2 ζ2 (MkMutResult t (MkSymbolicState pc2 δ2 h2) x)) =>
+               forall (ι' : SymInstance Σ2),
+                 ι = env_map (fun _ => inst_term ι') ζ2 ->
+                 let post__pc   := !! inst_pathcondition ι' pc2 in
+                 let post__heap := inst_heap ι' h2 in
+                 post__pc ∧ post__heap ⊢ POST (inst_term ι' t) (inst_localstore ι' δ2)) ->
+          δ ⊢ ⦃ pre__pc ∧ pre__heap ⦄ s ⦃ POST ⦄.
+      Proof.
+        intros ? ? ? ? ? ? ?; cbn.
+        revert pc1 h1.
+        induction s.
 
-      - intros.
-        apply rule_stm_lit.
-        apply H.
-        admit.
-
-      - intros.
-        apply rule_stm_exp.
-        rewrite eval_exp_inst.
-        apply H.
-        admit.
-
-      - cbn.
-        unfold dmut_bind_right, dmut_sub, dmut_bind; cbn.
-        repeat
-          (repeat setoid_rewrite outcome_satisfy_bind;
-           repeat setoid_rewrite outcome_satisfy_map; cbn).
-        repeat
-          (repeat setoid_rewrite sub_comp_id_left at 1;
-           repeat setoid_rewrite sub_comp_id_right at 1;
-           repeat setoid_rewrite subst_sub_id at 1;
-           cbn).
-        cbn.
-        intros.
-
-        eapply rule_stm_let.
-        + apply IHs1.
-          refine (outcome_satisfy_monotonic _ _ H); clear H. intros ?.
-          unfold dmut_bind_right, dmut_sub, dmut_bind; cbn.
-          rewrite ?outcome_satisfy_bind, ?outcome_satisfy_map; cbn.
-          intros.
+        - intros.
+          apply rule_stm_lit.
+          apply H.
           admit.
-        + admit.
-      - admit.
-      - admit.
-      - admit.
-      - admit.
-      - admit.
-      - cbn.
-        unfold dmut_bind_right, dmut_sub, dmut_bind; cbn.
-        repeat
-          (repeat setoid_rewrite outcome_satisfy_bind;
-           repeat setoid_rewrite outcome_satisfy_map; cbn).
-        repeat
-          (repeat setoid_rewrite sub_comp_id_left at 1;
-           repeat setoid_rewrite sub_comp_id_right at 1;
-           repeat setoid_rewrite subst_sub_id at 1;
-           cbn).
-        cbn.
-        cbv [mutator_assume_term mutator_assume_formula].
-        intros ? ? [H1 H2].
-        apply rule_stm_if.
-        + clear IHs2 H2.
-          revert H1.
-          destruct (try_solve_formula (formula_bool (symbolic_eval_exp δ1 e))) eqn:Heqfml.
-          * destruct (try_solve_formula_spec Term_eqb_spec (formula_bool (symbolic_eval_exp δ1 e)) Heqfml ι).
-            -- unfold mutator_pure; cbn.
-               repeat
-                 (repeat setoid_rewrite outcome_satisfy_bind;
-                  repeat setoid_rewrite outcome_satisfy_map; cbn).
-               repeat
-                 (repeat setoid_rewrite sub_comp_id_left at 1;
-                  repeat setoid_rewrite sub_comp_id_right at 1;
-                  repeat setoid_rewrite subst_sub_id at 1;
-                  cbn).
-               intros H1.
-               eapply rule_consequence; [ idtac | idtac | apply IHs1 ]; clear IHs1.
-               apply land_left1. apply entails_refl.
-               intros; apply entails_refl.
-               admit.
-               (* refine (outcome_satisfy_monotonic _ _ H1); clear H1. *)
-               (* intros [Σ2 ζ2 [t2 [pc2 δ2 h2] oblig2]]; cbn; intros. *)
-               (* apply H. *)
-               (* now rewrite sub_comp_id_left. *)
-            -- intros H1; clear H1.
-               cbn in n.
-               unfold is_true in n.
-               rewrite eval_exp_inst.
-               destruct (inst_term ι (symbolic_eval_exp δ1 e)) eqn:?; try contradiction.
-               clear n.
-               clear Heqfml.
-               admit.
-          * unfold mutator_modify, mutator_state; cbn.
-            repeat
-              (repeat setoid_rewrite outcome_satisfy_bind;
-               repeat setoid_rewrite outcome_satisfy_map; cbn).
-            repeat
-              (repeat setoid_rewrite sub_comp_id_left at 1;
-               repeat setoid_rewrite sub_comp_id_right at 1;
-               repeat setoid_rewrite subst_sub_id at 1;
-               cbn).
-            intro.
+
+        - intros.
+          apply rule_stm_exp.
+          rewrite eval_exp_inst.
+          apply H.
+          admit.
+
+        - cbn.
+          unfold dmut_bind_right, dmut_sub, dmut_bind; cbn.
+          repeat
+            (repeat setoid_rewrite outcome_satisfy_bind;
+             repeat setoid_rewrite outcome_satisfy_map; cbn).
+          repeat
+            (repeat setoid_rewrite sub_comp_id_left at 1;
+             repeat setoid_rewrite sub_comp_id_right at 1;
+             repeat setoid_rewrite subst_sub_id at 1;
+             cbn).
+          cbn.
+          intros.
+
+          eapply rule_stm_let.
+          + apply IHs1.
+            refine (outcome_satisfy_monotonic _ _ H); clear H. intros ?.
+            unfold dmut_bind_right, dmut_sub, dmut_bind; cbn.
+            rewrite ?outcome_satisfy_bind, ?outcome_satisfy_map; cbn.
+            intros.
             admit.
-            (* eapply rule_consequence; *)
-            (*   [ idtac *)
-            (*   | idtac *)
-            (*   | apply IHs1; refine (outcome_satisfy_monotonic _ _ H1) *)
-            (*   ]; clear H1 IHs1. *)
-            (* admit. *)
-            (* intros; apply entails_refl. *)
-            (* cbn. *)
-            (* intros [Σ2 ζ2 [t2 [pc2 δ2 h2] oblig2]]; cbn; intros. *)
-    Admitted.
+          + admit.
+        - admit.
+        - admit.
+        - admit.
+        - admit.
+        - admit.
+        - cbn.
+          unfold dmut_bind_right, dmut_sub, dmut_bind; cbn.
+          repeat
+            (repeat setoid_rewrite outcome_satisfy_bind;
+             repeat setoid_rewrite outcome_satisfy_map; cbn).
+          repeat
+            (repeat setoid_rewrite sub_comp_id_left at 1;
+             repeat setoid_rewrite sub_comp_id_right at 1;
+             repeat setoid_rewrite subst_sub_id at 1;
+             cbn).
+          cbn.
+          cbv [mutator_assume_term mutator_assume_formula].
+          intros ? ? [H1 H2].
+          apply rule_stm_if.
+          + clear IHs2 H2.
+            revert H1.
+            destruct (try_solve_formula (formula_bool (symbolic_eval_exp δ1 e))) eqn:Heqfml.
+            * destruct (try_solve_formula_spec Term_eqb_spec (formula_bool (symbolic_eval_exp δ1 e)) Heqfml ι).
+              -- unfold mutator_pure; cbn.
+                 repeat
+                   (repeat setoid_rewrite outcome_satisfy_bind;
+                    repeat setoid_rewrite outcome_satisfy_map; cbn).
+                 repeat
+                   (repeat setoid_rewrite sub_comp_id_left at 1;
+                    repeat setoid_rewrite sub_comp_id_right at 1;
+                    repeat setoid_rewrite subst_sub_id at 1;
+                    cbn).
+                 intros H1.
+                 eapply rule_consequence; [ idtac | idtac | apply IHs1 ]; clear IHs1.
+                 apply land_left1. apply entails_refl.
+                 intros; apply entails_refl.
+                 admit.
+                 (* refine (outcome_satisfy_monotonic _ _ H1); clear H1. *)
+                 (* intros [Σ2 ζ2 [t2 [pc2 δ2 h2] oblig2]]; cbn; intros. *)
+                 (* apply H. *)
+                 (* now rewrite sub_comp_id_left. *)
+              -- intros H1; clear H1.
+                 cbn in n.
+                 unfold is_true in n.
+                 rewrite eval_exp_inst.
+                 destruct (inst_term ι (symbolic_eval_exp δ1 e)) eqn:?; try contradiction.
+                 clear n.
+                 clear Heqfml.
+                 admit.
+            * unfold mutator_modify, mutator_state; cbn.
+              repeat
+                (repeat setoid_rewrite outcome_satisfy_bind;
+                 repeat setoid_rewrite outcome_satisfy_map; cbn).
+              repeat
+                (repeat setoid_rewrite sub_comp_id_left at 1;
+                 repeat setoid_rewrite sub_comp_id_right at 1;
+                 repeat setoid_rewrite subst_sub_id at 1;
+                 cbn).
+              intro.
+              admit.
+              (* eapply rule_consequence; *)
+              (*   [ idtac *)
+              (*   | idtac *)
+              (*   | apply IHs1; refine (outcome_satisfy_monotonic _ _ H1) *)
+              (*   ]; clear H1 IHs1. *)
+              (* admit. *)
+              (* intros; apply entails_refl. *)
+              (* cbn. *)
+              (* intros [Σ2 ζ2 [t2 [pc2 δ2 h2] oblig2]]; cbn; intros. *)
+      Admitted.
 
-    Lemma dmut_contract_sound {Δ τ} (c : SepContract Δ τ) (body : Stm Δ τ) :
-      ValidContractDynMut c body ->
-      ValidContract c body.
-    Proof.
-    Admitted.
+      Lemma dmut_contract_sound {Δ τ} (c : SepContract Δ τ) (body : Stm Δ τ) :
+        ValidContractDynMut c body ->
+        ValidContract c body.
+      Proof.
+      Admitted.
 
-  End Soundness.
+    End WithSemantics.
+
+  End DynMutV1Soundness.
 
 End Soundness.
